src/HOL/BNF/Examples/Derivation_Trees/DTree.thy
@@ -1,0 +1,95 @@
+(*  Title:      HOL/BNF/Examples/Infinite_Derivation_Trees/DTree.thy
+    Author:     Andrei Popescu, TU Muenchen
+    Copyright   2012
+
+Derivation trees with nonterminal internal nodes and terminal leaves.
+*)
+
+header {* Trees with Nonterminal Internal Nodes and Terminal Leaves *}
+
+theory DTree
+imports Prelim
+begin
+
+hide_fact (open) Quotient_Product.prod_rel_def
+
+typedecl N
+typedecl T
+
+codata dtree = NNode (root: N) (ccont: "(T + dtree) fset")
+
+
+subsection{* The characteristic lemmas transported from fset to set *}
+
+definition "Node n as \<equiv> NNode n (the_inv fset as)"
+definition "cont \<equiv> fset o ccont"
+definition "unfold rt ct \<equiv> dtree_unfold rt (the_inv fset o ct)"
+definition "corec rt qt ct dt \<equiv> dtree_corec rt qt (the_inv fset o ct) (the_inv fset o dt)"
+
+lemma finite_cont[simp]: "finite (cont tr)"
+unfolding cont_def by auto
+
+lemma Node_root_cont[simp]:
+"Node (root tr) (cont tr) = tr"
+using dtree.collapse unfolding Node_def cont_def
+by (metis cont_def finite_cont fset_cong fset_to_fset o_def)
+
+lemma dtree_simps[simp]:
+assumes "finite as" and "finite as'"
+shows "Node n as = Node n' as' \<longleftrightarrow> n = n' \<and> as = as'"
+using assms dtree.inject unfolding Node_def
+by (metis fset_to_fset)
+
+lemma dtree_cases[elim, case_names Node Choice]:
+assumes Node: "\<And> n as. \<lbrakk>finite as; tr = Node n as\<rbrakk> \<Longrightarrow> phi"
+shows phi
+apply(cases rule: dtree.exhaust[of tr])
+using Node unfolding Node_def
+by (metis Node Node_root_cont finite_cont)
+
+lemma dtree_sel_ctor[simp]:
+"root (Node n as) = n"
+"finite as \<Longrightarrow> cont (Node n as) = as"
+unfolding Node_def cont_def by auto
+
+lemmas root_Node = dtree_sel_ctor(1)
+lemmas cont_Node = dtree_sel_ctor(2)
+
+lemma dtree_cong:
+assumes "root tr = root tr'" and "cont tr = cont tr'"
+shows "tr = tr'"
+by (metis Node_root_cont assms)
+
+lemma set_rel_cont: 
+"set_rel \<chi> (cont tr1) (cont tr2) = fset_rel \<chi> (ccont tr1) (ccont tr2)"
+unfolding cont_def comp_def fset_rel_fset ..
+
+lemma dtree_coinduct[elim, consumes 1, case_names Lift, induct pred: "HOL.eq"]:
+assumes phi: "\<phi> tr1 tr2" and
+Lift: "\<And> tr1 tr2. \<phi> tr1 tr2 \<Longrightarrow>
+                  root tr1 = root tr2 \<and> set_rel (sum_rel op = \<phi>) (cont tr1) (cont tr2)"
+shows "tr1 = tr2"
+using phi apply(elim dtree.coinduct)
+apply(rule Lift[unfolded set_rel_cont]) . 
+ 
+lemma unfold:
+"root (unfold rt ct b) = rt b"
+"finite (ct b) \<Longrightarrow> cont (unfold rt ct b) = image (id \<oplus> unfold rt ct) (ct b)"
+using dtree.sel_unfold[of rt "the_inv fset \<circ> ct" b] unfolding unfold_def
+apply - apply metis
+unfolding cont_def comp_def
+by (metis (no_types) fset_to_fset map_fset_image)
+
+lemma corec:
+"root (corec rt qt ct dt b) = rt b"
+"\<lbrakk>finite (ct b); finite (dt b)\<rbrakk> \<Longrightarrow>
+ cont (corec rt qt ct dt b) =
+ (if qt b then ct b else image (id \<oplus> corec rt qt ct dt) (dt b))"
+using dtree.sel_corec[of rt qt "the_inv fset \<circ> ct" "the_inv fset \<circ> dt" b] 
+unfolding corec_def
+apply -
+apply simp
+unfolding cont_def comp_def id_def
+by (metis (no_types) fset_to_fset map_fset_image)
+
+end
