src/HOL/BNF/More_BNFs.thy
@@ -470,6 +470,9 @@ next
   unfolding fset_rel_def fset_rel_aux by simp
 qed auto
 
+lemma fset_rel_fset: "set_rel \<chi> (fset A1) (fset A2) = fset_rel \<chi> A1 A2"
+unfolding fset_rel_def set_rel_def by auto 
+
 (* Countable sets *)
 
 lemma card_of_countable_sets_range:
@@ -1507,5 +1510,77 @@ using  multiset_rel_imp_multiset_rel' multiset_rel'_imp_multiset_rel by auto
 (* The main end product for multiset_rel: inductive characterization *)
 theorems multiset_rel_induct[case_names empty add, induct pred: multiset_rel] =
          multiset_rel'.induct[unfolded multiset_rel_multiset_rel'[symmetric]]
+
+
+
+(* Advanced relator customization *)
+
+(* Set vs. sum relators: *)
+(* FIXME: All such facts should be declared as simps: *)
+declare sum_rel_simps[simp]
+
+lemma set_rel_sum_rel[simp]: 
+"set_rel (sum_rel \<chi> \<phi>) A1 A2 \<longleftrightarrow> 
+ set_rel \<chi> (Inl -` A1) (Inl -` A2) \<and> set_rel \<phi> (Inr -` A1) (Inr -` A2)"
+(is "?L \<longleftrightarrow> ?Rl \<and> ?Rr")
+proof safe
+  assume L: "?L"
+  show ?Rl unfolding set_rel_def Bex_def vimage_eq proof safe
+    fix l1 assume "Inl l1 \<in> A1"
+    then obtain a2 where a2: "a2 \<in> A2" and "sum_rel \<chi> \<phi> (Inl l1) a2"
+    using L unfolding set_rel_def by auto
+    then obtain l2 where "a2 = Inl l2 \<and> \<chi> l1 l2" by (cases a2, auto)
+    thus "\<exists> l2. Inl l2 \<in> A2 \<and> \<chi> l1 l2" using a2 by auto
+  next
+    fix l2 assume "Inl l2 \<in> A2"
+    then obtain a1 where a1: "a1 \<in> A1" and "sum_rel \<chi> \<phi> a1 (Inl l2)"
+    using L unfolding set_rel_def by auto
+    then obtain l1 where "a1 = Inl l1 \<and> \<chi> l1 l2" by (cases a1, auto)
+    thus "\<exists> l1. Inl l1 \<in> A1 \<and> \<chi> l1 l2" using a1 by auto
+  qed
+  show ?Rr unfolding set_rel_def Bex_def vimage_eq proof safe
+    fix r1 assume "Inr r1 \<in> A1"
+    then obtain a2 where a2: "a2 \<in> A2" and "sum_rel \<chi> \<phi> (Inr r1) a2"
+    using L unfolding set_rel_def by auto
+    then obtain r2 where "a2 = Inr r2 \<and> \<phi> r1 r2" by (cases a2, auto)
+    thus "\<exists> r2. Inr r2 \<in> A2 \<and> \<phi> r1 r2" using a2 by auto
+  next
+    fix r2 assume "Inr r2 \<in> A2"
+    then obtain a1 where a1: "a1 \<in> A1" and "sum_rel \<chi> \<phi> a1 (Inr r2)"
+    using L unfolding set_rel_def by auto
+    then obtain r1 where "a1 = Inr r1 \<and> \<phi> r1 r2" by (cases a1, auto)
+    thus "\<exists> r1. Inr r1 \<in> A1 \<and> \<phi> r1 r2" using a1 by auto
+  qed
+next
+  assume Rl: "?Rl" and Rr: "?Rr"
+  show ?L unfolding set_rel_def Bex_def vimage_eq proof safe
+    fix a1 assume a1: "a1 \<in> A1"
+    show "\<exists> a2. a2 \<in> A2 \<and> sum_rel \<chi> \<phi> a1 a2"
+    proof(cases a1)
+      case (Inl l1) then obtain l2 where "Inl l2 \<in> A2 \<and> \<chi> l1 l2"
+      using Rl a1 unfolding set_rel_def by blast
+      thus ?thesis unfolding Inl by auto
+    next
+      case (Inr r1) then obtain r2 where "Inr r2 \<in> A2 \<and> \<phi> r1 r2"
+      using Rr a1 unfolding set_rel_def by blast
+      thus ?thesis unfolding Inr by auto
+    qed
+  next
+    fix a2 assume a2: "a2 \<in> A2"
+    show "\<exists> a1. a1 \<in> A1 \<and> sum_rel \<chi> \<phi> a1 a2"
+    proof(cases a2)
+      case (Inl l2) then obtain l1 where "Inl l1 \<in> A1 \<and> \<chi> l1 l2"
+      using Rl a2 unfolding set_rel_def by blast
+      thus ?thesis unfolding Inl by auto
+    next
+      case (Inr r2) then obtain r1 where "Inr r1 \<in> A1 \<and> \<phi> r1 r2"
+      using Rr a2 unfolding set_rel_def by blast
+      thus ?thesis unfolding Inr by auto
+    qed
+  qed
+qed
+
+
+
 
 end
